proved up to call to findnext

concurrency/templates/coupling_lib_mixed.v
@@ -2,10 +2,11 @@ Require Import VST.concurrency.conclib.
 Require Import VST.floyd.proofauto.
 Require Import VST.floyd.library.
 Require Import VST.atomics.general_locks. 
-Require Export VST.atomics.verif_lock_atomic.
+Require Import VST.atomics.verif_lock_atomic.
 Require Import VST.concurrency.semax_conc.
 Require Import bst.puretree.
-From refinedc.project.rc.bst_template_coupling Require Import generated_code.
+From refinedc.project.rc.bst_template_coupling Require Import generated_code generated_spec.
+From iris.algebra Require Import auth gset excl.
 
 Section TREES.
   Context { V : Type }.
@@ -43,9 +44,6 @@ match s with
 end.
 
 End TREES.
-
-#[export] Instance CompSpecs : compspecs. make_compspecs prog. Defined.
-Definition Vprog : varspecs. mk_varspecs prog. Defined.
 
 Definition t_struct_tree := Tstruct _tree noattr.
 Definition t_struct_tree_t := Tstruct _tree_t noattr.
@@ -102,9 +100,9 @@ Proof.
   apply ra_total_mixin; try done.
   - by intros ??? ->.
   - by intros ?? ->.
-  - intros ???. symmetry; apply merge_assoc.
-  - intros ??. apply merge_comm.
-  - intros ?. apply merge_id.
+  - intros ???. symmetry; apply puretree.merge_assoc.
+  - intros ??. apply puretree.merge_comm.
+  - intros ?. apply puretree.merge_id.
 Qed.
 Canonical Structure rangeR := discreteR range range_ra_mixin.
 
@@ -117,14 +115,12 @@ Proof.
 Qed.
 Canonical Structure rangeUR := Ucmra range range_ucmra_mixin.
 
-From iris.algebra Require Import auth gset.
-
 Definition ghost_ref `{!inG Σ (ext_order.inclR (authR (gsetUR gname)))} g r1 := own(inG0 := inG0) g (● r1).
 
 Definition in_tree `{!inG Σ (ext_order.inclR (authR (gsetUR gname)))} g r1 := own(inG0 := inG0) g (◯ {[r1]}).
 
 (*Lemma in_tree_add : forall g s g1 g', ~Ensembles.In s g' -> in_tree g g1 * ghost_ref g s 
-  |-- (|==> !! (g1 <> g') && (ghost_ref g (Add s g') * in_tree g g1 * in_tree g g'))%I.
+  ⊢ (|==> !! (g1 <> g') && (ghost_ref g (Add s g') * in_tree g g1 * in_tree g g'))%I.
 Proof.
   intros.
   unfold in_tree at 1. Intros sh. iIntros "H".
@@ -158,19 +154,18 @@ Proof.
     inv H5; inv H6; contradiction.
   * intro; contradiction H2; eapply Share.split_nontrivial; eauto.
   * intro; contradiction H2; eapply Share.split_nontrivial; eauto.
-Qed.
-
+Qed.*)
 
 Definition ghost_info : Type := (key * val * gname * gname)%type.
 
 (* This allows the range to be outdated while the ghost_info may be present or absent. *)
-#[export] Instance node_ghost : Ghost := prod_PCM range_ghost (exclusive_PCM (option ghost_info)).
+Definition nodeR := prodR rangeR (optionR (exclR (option ghost_info))).
 
-Notation node_info := (@G node_ghost).
+Notation node_info := (cmra_car nodeR).
 
-Lemma ghost_node_alloc : forall g s g1 (a : node_info),
-  finite s -> in_tree g g1 * ghost_ref g s |-- 
-    (|==> EX g', !! (¬ Ensembles.In s g' /\ g1 <> g') &&
+(*Lemma ghost_node_alloc : forall g s g1 (a : node_info),
+  finite s -> in_tree g g1 * ghost_ref g s ⊢ 
+    (|==> ∃ g', !! (¬ Ensembles.In s g' /\ g1 <> g') &&
                    (both_halves a g' * ghost_ref g (Add s g') * in_tree g g1 * in_tree g g'))%I.
 Proof.
   intros.
@@ -188,7 +183,7 @@ Proof.
   { apply @part_ref_valid. }
   iExists g'. iFrame.
   iMod (in_tree_add _ _ _ g' with "r") as "(% & ($ & $))"; auto.
-Qed.
+Qed.*)
 
 Lemma gsh1_not_Tsh : gsh1 <> Tsh.
 Proof.
@@ -203,62 +198,85 @@ Proof.
 Qed.
 Global Hint Resolve gsh1_not_Tsh gsh2_not_Tsh : core.
 
-Lemma range_incl_join: forall  (r1 r2 r3 : node_info), sepalg.join r1 r2 r3 -> range_incl r1.1 r3.1 = true /\ range_incl r2.1 r3.1 = true.
+(*Lemma range_incl_join: forall  (r1 r2 r3 : node_info), sepalg.join r1 r2 r3 -> range_incl r1.1 r3.1 = true /\ range_incl r2.1 r3.1 = true.
 Proof.
   intros. destruct r1 as [range1 r1]. destruct r2 as [range2 r2]. destruct r3 as [range3 r3].
   hnf in H. simpl in *. destruct H. inv H; auto. split; [|rewrite merge_comm]; eapply merge_range_incl; eauto.
-Qed.
+Qed.*)
+
+Section inv.
+Context `{!VSTGS OK_ty Σ, !cinvG Σ, atom_impl : !atomic_int_impl (Tstruct threads._atom_int noattr)}
+  `{!inG Σ (ext_order.inclR (authR (gsetUR gname)))} `{!inG Σ (frac_auth.frac_authR nodeR)} `{!cinvG Σ}.
 
 (* Each lock will hold gsh1 of my_half, with gsh2 held by the invariant, allowing the lock's range to become outdated.
   The exception is the root node, which will hold some smaller fraction of gsh1, allowing clients to know that the root's range is total. *)
 
 (* base definition for node_lock_inv_r *)
 
-Definition node_lock_inv_r' (R : (val * (own.gname * node_info) → mpred)) sh p gp lock :=
-  sync_inv gp sh (curry (curry R p))  *
+Definition node_lock_inv_r' (R : (val * (gname * node_info) -d> mpred)) : Qp -d> val -d> gname -d> val -d> mpred :=
+  λ sh p gp lock,
+  sync_inv gp sh (curry (curry R p)) ∗
   field_at lsh2 t_struct_tree_t [StructField _lock] lock p (* *
   malloc_token Ews t_lock lock*).
 
-Definition node_lock_inv_r (R : (val * (own.gname * node_info) → mpred)) sh p gp lock:=
-      selflock (node_lock_inv_r' R sh p gp (ptr_of lock)) gsh2 lock.
+Local Instance node_lock_inv_r'_ne : NonExpansive node_lock_inv_r'.
+Proof. repeat intro. rewrite /node_lock_inv_r' /sync_inv. do 6 f_equiv.
+  intros ?? ->%discrete; last apply _. done. Qed.
+
+Definition node_lock_inv_r (R : (val * (gname * node_info) -d> mpred)) : Qp -d> val -d> gname -d> lock_handle -d> mpred :=
+  λ sh p gp lock, selflock (node_lock_inv_r' R sh p gp (ptr_of lock)) (1/2) lock.
+
+Local Instance node_lock_inv_r_ne : NonExpansive node_lock_inv_r.
+Proof. repeat intro. rewrite /node_lock_inv_r /selflock. f_equiv. by apply node_lock_inv_r'_ne. Qed.
 
 (* fix share
    sh - for field_at
    ish - for lock_inv
    gsh - for node_lock_inv
  *)
-Definition ltree_r R (g_root:gname) sh ish gsh p lock :=
-  !!(field_compatible t_struct_tree_t nil p) &&
-  (field_at sh t_struct_tree_t [StructField _lock] (ptr_of lock) p *
+Definition ltree_r R : gname -d> share -d> Qp -d> Qp -d> val -d> lock_handle -d> mpred :=
+λ g_root sh ish gsh p lock,
+  ⌜field_compatible t_struct_tree_t nil p⌝ ∧
+  (field_at sh t_struct_tree_t [StructField _lock] (ptr_of lock) p ∗
    lock_inv ish lock (node_lock_inv_r R gsh p g_root lock)).
+
+Local Instance ltree_r_ne : NonExpansive ltree_r.
+Proof. repeat intro. rewrite /ltree_r. do 3 f_equiv. by apply node_lock_inv_r_ne. Qed.
 
 (* Does the range ghost help at all, given that we could calculate it precisely from the nodes we've seen?
   Yes, since the nodes we've seen may change after we pass them. *)
 
 
-Definition node_rep_r (g:gname) R arg : mpred := 
+Definition node_rep_r (g:gname) (R : val * (gname * node_info) -d> mpred) : (val * (gname * node_info)) -d> mpred := λ arg,
   let '(np, (g_current,(r,g_info))) := arg in
-EX tp:val,
-(field_at Ews (t_struct_tree_t) [StructField _t] tp np) *
- malloc_token Ews t_struct_tree_t np * in_tree g g_current *
+∃ tp:val,
+(field_at Ews (t_struct_tree_t) [StructField _t] tp np) ∗
+ malloc_token Ews t_struct_tree_t np ∗ in_tree g g_current ∗
 if eq_dec tp nullval 
-then !!(g_info = Some None) && seplog.emp  
+then ⌜g_info = Excl' None⌝ ∧ emp  
 else
-EX ga:gname, EX gb: gname, EX x: Z, EX v: val, EX pa : val, EX pb : val, EX (locka lockb : lock_handle),
-     !! (g_info = Some (Some(x,v,ga,gb)) /\ 
+∃ ga:gname, ∃ gb: gname, ∃ x: Z, ∃ v: val, ∃ pa : val, ∃ pb : val, ∃ (locka lockb : lock_handle),
+     ⌜g_info = Excl' (Some(x,v,ga,gb)) /\ 
      and (Z.le Int.min_signed x) (Z.le x Int.max_signed) /\ 
      is_pointer_or_null pa /\ is_pointer_or_null pb  /\ tc_val (tptr Tvoid) v
-     /\ key_in_range x r = true) && 
-     data_at Ews t_struct_tree (Vint (Int.repr x),(v,(pa,pb))) tp * 
-     malloc_token Ews t_struct_tree tp  *
-    |> ltree_r R ga lsh1 gsh1 gsh1 pa locka * |> ltree_r R gb lsh1 gsh1 gsh1 pb lockb.
+     /\ key_in_range x r = true⌝ ∧
+     data_at Ews t_struct_tree (Vint (Int.repr x),(v,(pa,pb))) tp ∗
+     malloc_token Ews t_struct_tree tp ∗
+    ▷ ltree_r R ga lsh1 (1/2)%Qp (1/2)%Qp pa locka ∗ ▷ ltree_r R gb lsh1 (1/2)%Qp (1/2)%Qp pb lockb.
 
-Definition node_rep_closed g := HORec (node_rep_r g).
+Local Instance node_rep_r_contractive g : Contractive (node_rep_r g).
+Proof.
+  rewrite /node_rep_r => n ???.
+  intros (?, (?, (?, ?))).
+  do 26 f_equiv; f_contractive; by apply ltree_r_ne.
+Qed.
+
+Definition node_rep_closed g := fixpoint (node_rep_r g).
 
 Definition node_rep np g g_current r := node_rep_closed g (np, (g_current, r)).
 
 Definition node_lock_inv_pred sh g p gp lock :=
-  sync_inv gp sh (node_rep p g) *
+  sync_inv gp sh (node_rep p g) ∗
   field_at lsh2 t_struct_tree_t [StructField _lock] lock p
  (* * 
   malloc_token Ews t_lock lock
@@ -266,18 +284,23 @@ Definition node_lock_inv_pred sh g p gp lock :=
 (* No malloc token for t_struct_tree_t because node_rep_r contains one *)
 
 Definition node_lock_inv sh g p gp lock :=
-  selflock (node_lock_inv_pred sh g p gp (ptr_of lock)) gsh2 lock.
+  selflock (node_lock_inv_pred sh g p gp (ptr_of lock)) (1/2) lock.
 
-Definition public_half' (g : gname) (d : range * option (option ghost_info)) := 
-  my_half g gsh2 (fst d, None) * public_half g d.
+Definition ltree (g : gname) (g_root : gname) sh ish gsh p lock :=
+  ⌜field_compatible t_struct_tree_t nil p⌝ ∧
+  (field_at sh t_struct_tree_t [StructField _lock] (ptr_of lock) p ∗
+     lock_inv ish lock (node_lock_inv gsh g p g_root lock)).
+
+Definition public_half' (g : gname) (d : range * excl' (option ghost_info)) := 
+  my_half g (1/2) (fst d, None) ∗ public_half g d.
 
  Fixpoint ghost_tree_rep (t: @ ghost_tree val) (g:gname) range : mpred :=
  match t, range with
- | E_ghost , _ => public_half' g (range, Some (@None ghost_info))
- | T_ghost a ga x v b gb, (l, r) => public_half' g (range, Some (Some (x,v,ga,gb))) * ghost_tree_rep a ga (l, Finite_Integer x) * ghost_tree_rep b gb (Finite_Integer x, r)
+ | E_ghost , _ => public_half' g (range, Excl' (@None ghost_info))
+ | T_ghost a ga x v b gb, (l, r) => public_half' g (range, Excl' (Some (x,v,ga,gb))) ∗ ghost_tree_rep a ga (l, Finite_Integer x) ∗ ghost_tree_rep b gb (Finite_Integer x, r)
  end.
 
-Lemma public_half_range_incl : forall g r r' o, range_incl r r' = true -> public_half' g (r, o) |-- (|==> public_half' g (r', o))%I.
+(*Lemma public_half_range_incl : forall g r r' o, range_incl r r' = true -> public_half' g (r, o) ⊢ (|==> public_half' g (r', o))%I.
 Proof.
   intros.
   iIntros "H".
@@ -289,34 +312,24 @@ Proof.
   symmetry; rewrite merge_comm; apply merge_range_incl'.
   eapply range_incl_trans; eauto.
   inversion 1; reflexivity.
-Qed.
+Qed.*)
 
-Fixpoint find_ghost_set (t : @ghost_tree val) (g:gname) : Ensemble gname :=
+Fixpoint find_ghost_set (t : @ghost_tree val) (g:gname) : gset gname :=
   match t with
-  | E_ghost => Ensembles.Singleton g
-  | T_ghost a ga x v  b gb => Add  (Union (find_ghost_set a ga) (find_ghost_set b gb)) g
+  | E_ghost => {[g]}
+  | T_ghost a ga x v  b gb => {[g]} ∪ find_ghost_set a ga ∪ find_ghost_set b gb
 end.
 
-Definition find_ghost_set' (t : @ghost_tree val) : Ensemble gname :=
+Definition find_ghost_set' (t : @ghost_tree val) :=
   match t with
-  | E_ghost => Empty_set
-  | T_ghost a ga x v  b gb => Union (find_ghost_set a ga) (find_ghost_set b gb)
+  | E_ghost => ∅
+  | T_ghost a ga x v  b gb => find_ghost_set a ga ∪ find_ghost_set b gb
 end.
-
-Lemma find_ghost_set_finite : forall t g, finite (find_ghost_set t g).
-Proof.
-  induction t; intros; simpl.
-  - apply finite_singleton.
-  - apply finite_add, finite_union; auto.
-Qed.
 
 Lemma find_ghost_set_equiv : forall t g,
-  find_ghost_set t g = Add (find_ghost_set' t) g.
+  find_ghost_set t g = {[g]} ∪ find_ghost_set' t.
 Proof.
-  intros. destruct t.
-  - unfold Add; simpl.
-    now rewrite invariants.Union_Empty.
-  - simpl; auto.
+  intros. destruct t; simpl; set_solver.
 Qed.
 
 Inductive unique_gname : ghost_tree -> Prop :=
@@ -324,11 +337,11 @@ Inductive unique_gname : ghost_tree -> Prop :=
   | Unique_Tree : forall (x : key) (v : val) (l : ghost_tree) (g1 : gname) (r : ghost_tree) (g2 : gname),
                   unique_gname l -> unique_gname r ->
                   g1 <> g2 ->
-                  Intersection (find_ghost_set' l) (find_ghost_set' r) = Empty_set ->
-                  ~Ensembles.In (find_ghost_set' l) g1 ->
-                  ~Ensembles.In (find_ghost_set' r) g1 ->
-                  ~Ensembles.In (find_ghost_set' r) g2 ->
-                  ~Ensembles.In (find_ghost_set' l) g2 ->
+                  find_ghost_set' l ∩ find_ghost_set' r = ∅ ->
+                  ~g1 ∈ (find_ghost_set' l) ->
+                  ~g1 ∈ (find_ghost_set' r) ->
+                  ~g2 ∈ (find_ghost_set' r) ->
+                  ~g2 ∈ (find_ghost_set' l) ->
                   unique_gname (T_ghost l g1 x v r g2).
 
 (* turn a tree into a gmap *)
@@ -338,120 +351,56 @@ Fixpoint tree_to_gmap (t : @ghost_tree val) : gmap key val :=
   | T_ghost a ga x v b gb => base.insert x v (union (tree_to_gmap a) (tree_to_gmap b))
   end.
 
-Definition tree_rep (g : gname) (g_root : gname)  (m: gmap key val) : mpred := EX tg : ghost_tree,
-  !! (~ Ensembles.In (find_ghost_set' tg) g_root /\ unique_gname tg /\ sorted_ghost_tree tg /\ tree_to_gmap tg = m) &&
-  ghost_tree_rep tg g_root (Neg_Infinity, Pos_Infinity) * ghost_ref g (find_ghost_set tg g_root).
+Definition tree_rep (g : gname) (g_root : gname)  (m: gmap key val) : mpred := ∃ tg : ghost_tree,
+  ⌜~ g_root ∈ (find_ghost_set' tg) /\ unique_gname tg /\ sorted_ghost_tree tg /\ tree_to_gmap tg = m⌝ ∧
+  ghost_tree_rep tg g_root (Neg_Infinity, Pos_Infinity) ∗ ghost_ref g (find_ghost_set tg g_root).
 
 (* fix share
    sh - for field_at
    ish - for lock_inv
    gsh - for node_lock_inv
  *)
-Definition ltree (g : gname) (g_root : gname) sh ish gsh p lock :=
-  !!(field_compatible t_struct_tree_t nil p) &&
-  (field_at sh t_struct_tree_t [StructField _lock] (ptr_of lock) p  *
-     lock_inv ish lock (node_lock_inv gsh g p g_root lock)).
-
 
 (* nodebox_rep knows that the range of the root is -infinity to +infinity, but doesn't know the data. *)
 (* reduce share to something related to the sh argument *)
-Definition nodebox_rep (g : gname) (g_root : gname) (sh : share) (lock : lock_handle) (nb : val) :=
-  EX np: val, data_at sh (tptr (t_struct_tree_t)) np nb *
-                ltree g g_root sh sh (fst (Share.split gsh1)) np lock *
-                my_half g_root (snd (Share.split gsh1)) (Neg_Infinity, Pos_Infinity, None).
+Definition nodebox_rep (g : gname) (g_root : gname) (sh : share) sh' (lock : lock_handle) (nb : val) :=
+  ∃ np: val, data_at sh (tptr (t_struct_tree_t)) np nb ∗
+                ltree g g_root sh sh' (1/4) np lock ∗
+                my_half g_root (1/4) (Neg_Infinity, Pos_Infinity, None).
 
 Lemma my_half_range_inf : forall g sh1 sh2 r1 r2 o,
-    my_half g sh1 (r1, o) * my_half g sh2 (Neg_Infinity, Pos_Infinity, None) |--
-    my_half g sh1 (r2, o) * my_half g sh2 (Neg_Infinity, Pos_Infinity, None).
+    my_half g sh1 (r1, o) ∗ my_half g sh2 (Neg_Infinity, Pos_Infinity, None) ⊢
+    my_half g sh1 (r2, o) ∗ my_half g sh2 (Neg_Infinity, Pos_Infinity, None).
 Proof.
   intros.
-  iIntros "H"; iPoseProof (own_valid_2 with "H") as "%".
-  destruct H as ((a, ?) & [J ?] & ?); simpl in J.
-  destruct a as [(?, ?)|]; try contradiction.
-  destruct J as (? & ? & ? & ?).
-  unfold my_half; erewrite 2 ghost_part_join with
-                      (a := (Neg_Infinity, Pos_Infinity, o));
-  eauto with share; repeat constructor; simpl; hnf; rewrite merge_infinity; auto.
+  iIntros "H"; rewrite !my_half_join -!pair_op.
+  rewrite {2 5}/op /cmra_op /= /range_op !merge_infinity //.
 Qed.
 
-Definition tree_rep_R (tp:val) (r:(range)) (g_info: option (option ghost_info)) g : mpred :=
+Definition tree_rep_R (tp:val) (r:(range)) (g_info: excl' (option ghost_info)) g : mpred :=
   if eq_dec tp nullval
-  then !!(g_info = Some None) && seplog.emp
+  then ⌜g_info = Excl' None⌝ ∧ emp
   else
-  EX ga : gname, EX gb : gname, EX x : Z, EX v : val,
-            EX pa : val, EX pb : val, EX (locka lockb : lock_handle),
-     !!(g_info = Some (Some(x,v,ga,gb)) /\
+  ∃ ga : gname, ∃ gb : gname, ∃ x : Z, ∃ v : val,
+            ∃ pa : val, ∃ pb : val, ∃ (locka lockb : lock_handle),
+     ⌜g_info = Excl' (Some(x,v,ga,gb)) /\
           and (Z.le Int.min_signed x) (Z.le x Int.max_signed) /\
           is_pointer_or_null pa /\ is_pointer_or_null pb  /\ tc_val (tptr Tvoid) v
-     /\ key_in_range x r = true) &&
-       data_at Ews t_struct_tree (Vint (Int.repr x),(v,(pa,pb))) tp *
-       malloc_token Ews t_struct_tree tp *
-     |> ltree g ga lsh1 gsh1 gsh1 pa locka * |> ltree g gb lsh1 gsh1 gsh1 pb lockb.
-
-(* up *)
-Lemma eqp_subp : forall P Q, P <=> Q |-- P >=> Q.
-Proof.
-  intros; constructor.
-  apply subtypes.eqp_subp, predicates_hered.derives_refl.
-Qed.
-
-(* up *)
-Lemma selflock_nonexpansive2 : forall {A} (P Q : A -> mpred) sh p x,
-    (ALL x : _, |> (P x <=> Q x) |--
-    |> (selflock (P x) sh p <=> selflock (Q x) sh p)).
-Proof.
-  intros. apply allp_left with x. apply later_derives.
-  apply nonexpansive_entail with (F := fun P => selflock P sh p).
-  apply sepcon_nonexpansive, identity_nonexpansive; apply const_nonexpansive.
-Qed.
-
-Lemma lock_inv_node_lock_inv_r_nonexpansive:
-  ∀ (P Q : val * (own.gname * node_info) → mpred)
-    (sh gsh: share) (gp : own.gname) (p : val) (lock : lock_handle),
-    ALL x : val * (own.gname * node_info),
-    |> (P x <=> Q x)
-       |-- |> lock_inv sh lock (node_lock_inv_r P gsh p gp lock) >=>
-           |> lock_inv sh lock (node_lock_inv_r Q gsh p gp lock).
-Proof.
-  intros. eapply derives_trans, eqp_subp. eapply derives_trans, lock_inv_nonexpansive2.
-  apply allp_right. intros v. unfold node_lock_inv_r.
-  eapply derives_trans, selflock_nonexpansive2.
-  apply allp_right. intros ?.
-  unfold node_lock_inv_r'. unfold sync_inv, curry, Datatypes.curry.
-  rewrite <- later_allp; apply later_derives.
-  eapply eqp_sepcon, eqp_refl.
-  apply eqp_exp. intros (?, ?). apply allp_left with (p, (gp, (g, g0))).
-  apply eqp_sepcon; [apply derives_refl | apply eqp_refl].
-Qed.
-
-Lemma ltree_r_nonexpansive:
-  ∀ (P Q : val * (own.gname * node_info) → mpred)
-    (sh ish gsh: share) (gp : own.gname) (p : val) (lock : lock_handle),
-    ALL x : val * (own.gname * node_info),
-    |> (P x <=> Q x) |-- |> ltree_r P gp sh ish gsh p lock >=> |> ltree_r Q gp sh ish gsh p lock.
-Proof.
-  intros. unfold ltree_r. rewrite !later_andp. apply subp_andp; [apply subp_refl|].
-  rewrite !later_sepcon. apply subp_sepcon; [apply subp_refl|].
-  apply lock_inv_node_lock_inv_r_nonexpansive.
-Qed.
+     /\ key_in_range x r = true⌝ ∧
+       data_at Ews t_struct_tree (Vint (Int.repr x),(v,(pa,pb))) tp ∗
+       malloc_token Ews t_struct_tree tp ∗
+     ▷ ltree g ga lsh1 (1/2) (1/2) pa locka ∗ ▷ ltree g gb lsh1 (1/2) (1/2) pb lockb.
 
 Lemma node_rep_def : forall np r g g_current,
-    node_rep np g g_current r =
-    EX tp:val, (field_at Ews (t_struct_tree_t) [StructField _t] tp np) *
-               malloc_token Ews t_struct_tree_t np *  in_tree g g_current *
+    node_rep np g g_current r ≡
+    ∃ tp:val, (field_at Ews (t_struct_tree_t) [StructField _t] tp np) ∗
+               malloc_token Ews t_struct_tree_t np ∗ in_tree g g_current ∗
                tree_rep_R tp (fst r) (snd r) g.
 Proof.
-  intros. assert (HOcontractive (node_rep_r g)). {
-    apply prove_HOcontractive'. intros ?? (?, (?, (?, ?))). unfold node_rep_r.
-    apply subp_exp; intros. apply subp_sepcon; [apply subp_refl|].
-    destruct (eq_dec x nullval). 1: apply subp_refl. repeat (apply subp_exp; intro).
-    rewrite !sepcon_assoc; apply subp_sepcon; [apply subp_refl|].
-    apply subp_sepcon; [apply subp_refl|].
-    apply subp_sepcon; apply ltree_r_nonexpansive. }
-  unfold node_rep, node_rep_closed.
-  etransitivity; [eapply equal_f, HORec_fold_unfold|]; auto.
-  unfold node_rep_r at 1.
-  destruct r; reflexivity.
+  intros; rewrite /node_rep /node_rep_closed.
+  etrans; first apply (fixpoint_unfold (node_rep_r g)).
+  rewrite {1}/node_rep_r /tree_rep_R.
+  destruct r; repeat f_equiv; done.
 Qed.
 
 Lemma node_lock_inv_pred_exclusive : forall sh p lock g g_current,
@@ -461,29 +410,21 @@ Proof.
   unfold node_lock_inv_pred, sync_inv.
   eapply derives_exclusive, exclusive_sepcon1  with
   (P := field_at lsh2 t_struct_tree_t [StructField _lock] lock p)
-  (Q := (EX a : node_info, node_rep p g g_current a * my_half(P := node_ghost) g_current sh a)).
+  (Q := (∃ a : node_info, node_rep p g g_current a ∗ my_half g_current sh a)).
   - Intros a.
     Exists a. cancel.
   - apply field_at_exclusive; auto.
     simpl. lia.
 Qed.
-Global Hint Resolve node_lock_inv_pred_exclusive : core.
 
-Lemma node_exist_in_tree: forall g s g_in, in_tree g g_in * ghost_ref g s |--
-                                      !! (Ensembles.In s g_in).
+Lemma node_exist_in_tree: forall g s g_in, in_tree g g_in ∗ ghost_ref g s ⊢
+                                      ⌜g_in ∈ s⌝.
 Proof.
   intros.
-  unfold ghost_ref, in_tree; Intros sh.
-  rewrite ref_sub.
-  destruct  (eq_dec sh Tsh).
-  - Intros.
-    apply log_normalize.prop_derives. intros. subst s.
-    apply In_singleton.
-  - apply log_normalize.prop_derives. intros [m H].
-    unfold sepalg.join in H. hnf in H. destruct H.
-    rewrite H0.
-    apply Union_introl.
-    apply In_singleton.
+  unfold ghost_ref, in_tree.
+  rewrite -own_op own_valid ouPred.discrete_valid; f_equiv.
+  rewrite /impl comm auth_both_valid_discrete gset_included.
+  set_solver.
 Qed.
 
 Lemma In_tree_to_gmap : forall x t, In_ghost x t <-> tree_to_gmap t !! x <> None.
@@ -507,9 +448,9 @@ Qed.
 
 Inductive range_info_in_tree (ri: node_info)
           (range: range): ghost_tree -> Prop :=
-| riit_none: ri = (range, Some None) -> range_info_in_tree ri range E_ghost
+| riit_none: ri = (range, Excl' None) -> range_info_in_tree ri range E_ghost
 | riit_root: forall (l r: ghost_tree) (g1 g2: gname) k v,
-    ri = (range, Some (Some (k, v, g1, g2))) ->
+    ri = (range, Excl' (Some (k, v, g1, g2))) ->
     range_info_in_tree ri range (T_ghost l g1 k v r g2)
 | riit_left: forall (l r: ghost_tree) (g1 g2: gname) k v,
     range_info_in_tree ri (range.1, Finite_Integer k) l ->
@@ -518,11 +459,10 @@ Inductive range_info_in_tree (ri: node_info)
     range_info_in_tree ri (Finite_Integer k, range.2) r ->
     range_info_in_tree ri range (T_ghost l g1 k v r g2).
 
-Definition empty_range rn tg r_root := range_info_in_tree (rn, Some None) r_root tg.
+Definition empty_range rn tg r_root := range_info_in_tree (rn, Excl' None) r_root tg.
 
 Lemma empty_range_E : forall r, empty_range r E_ghost r.
 Proof. constructor; auto. Qed.
-Global Hint Resolve empty_range_E : core.
 
 Definition keys_in_range_ghost (t : @ghost_tree val) r := forall k,
     In_ghost k t -> key_in_range k r = true.
@@ -551,14 +491,12 @@ Lemma keys_in_range_infinity : forall tg, keys_in_range_ghost tg (Neg_Infinity, 
 Proof.
   intros ???; auto.
 Qed.
-Global Hint Resolve keys_in_range_infinity : core.
 
 Lemma ghost_range_inside_ghost_range : forall r r_root tg, empty_range r tg r_root -> keys_in_range_ghost tg r_root -> sorted_ghost_tree tg -> range_incl r r_root = true.
 Proof.
-  intros; revert dependent r_root.
+  intros; generalize dependent r_root.
   induction tg; intros; inv H.
-  - inv H2; apply range_incl_refl.
-  - inv H3.
+  - apply range_incl_refl.
   - eapply keys_in_range_ghost_subtrees in H0 as (? & ? & ?); [|auto].
     inv H1.
     eapply range_incl_trans; [apply IHtg1; eauto 1|].
@@ -579,7 +517,6 @@ Proof.
   { intros X; inv X. }
   apply keys_in_range_ghost_subtrees in Hrange as (? & ? & ?); [|auto].
   intros X. inv Hsorted. inv Hempty.
-  - inv H4.
   - exploit IHtg1; eauto.
     apply ghost_range_inside_ghost_range in H4; auto.
     eapply key_in_range_incl in H; eauto.
@@ -594,69 +531,73 @@ Proof.
     * specialize (Hgtl _ H5); simpl in H; lia.
 Qed.
 
-Lemma both_halves_join : forall g a, my_half g gsh1 a * public_half g a = both_halves a g.
+Global Instance range_core (a : rangeR): CoreId a.
+Proof. rewrite /CoreId //. Qed.
+
+Lemma both_halves_join : forall g a, my_half g (1/2) a ∗ public_half g a ⊣⊢ both_halves a g.
 Proof.
   intros; rewrite <- both_halves_join.
-  unfold public_half'; erewrite <- sepcon_assoc, my_half_join; eauto with share.
-  repeat constructor; hnf; simpl.
-  symmetry; apply merge_id.
+  unfold public_half'. rewrite sep_assoc my_half_join.
+  destruct a; rewrite -pair_op right_id.
+  rewrite /my_half -core_id_dup frac_op Qp.half_half //.
 Qed.
 
 Lemma ghost_tree_rep_public_half_ramif2: forall tg g_root r_root g_in,
-    Ensembles.In (find_ghost_set tg g_root) g_in ->
+    g_in ∈ (find_ghost_set tg g_root) ->
     ghost_tree_rep tg g_root r_root
-    |--
-    (EX r: range ,
-           (public_half g_in (r, Some (@None ghost_info)) *
-            (public_half g_in (r, Some (@None ghost_info)) -*
-                         ghost_tree_rep tg g_root r_root))) ||
-    (EX r: range, EX x: key, EX v: val, EX ga gb: gname,
-     EX i1 i2: option ghost_info,
-        ((public_half g_in (r, Some (Some (x, v, ga, gb))) *
-          public_half ga ((r.1, Finite_Integer x), Some i1) *
-          public_half gb ((Finite_Integer x, r.2), Some i2)) *
-        ((public_half g_in (r, Some (Some (x, v, ga, gb))) *
-          public_half ga ((r.1, Finite_Integer x), Some i1) *
-          public_half gb ((Finite_Integer x, r.2), Some i2))
-           -* ghost_tree_rep tg g_root r_root))).
+    ⊢
+    (∃ r: range ,
+           (public_half g_in (r, Excl' (@None ghost_info)) ∗
+            (public_half g_in (r, Excl' (@None ghost_info)) -∗
+                         ghost_tree_rep tg g_root r_root))) ∨
+    (∃ r: range, ∃ x: key, ∃ v: val, ∃ ga gb: gname,
+     ∃ i1 i2: option ghost_info,
+        ((public_half g_in (r, Excl' (Some (x, v, ga, gb))) ∗
+          public_half ga ((r.1, Finite_Integer x), Excl' i1) ∗
+          public_half gb ((Finite_Integer x, r.2), Excl' i2)) ∗
+        ((public_half g_in (r, Excl' (Some (x, v, ga, gb))) ∗
+          public_half ga ((r.1, Finite_Integer x), Excl' i1) ∗
+          public_half gb ((Finite_Integer x, r.2), Excl' i2))
+           -∗ ghost_tree_rep tg g_root r_root))).
 Proof.
   induction tg; intros; simpl in *.
-  - apply orp_right1. inv H. Exists r_root. cancel. apply wand_refl_cancel_right.
-  - destruct r_root as [lroot rroot]. inv H; inv H0.
-    + specialize (IHtg1 _ (lroot, Finite_Integer k) _ H). sep_apply IHtg1. clear.
-      rewrite distrib_orp_sepcon. apply orp_derives.
-      * Intros r. Exists r. cancel. rewrite <- wand_sepcon_adjoint.
-        cancel. apply wand_frame_elim''.
-      * Intros r x v0 ga gb i1 i2. Exists r x v0 ga gb i1 i2. cancel.
-        rewrite <- wand_sepcon_adjoint. cancel.
-        rewrite !sepcon_assoc. apply wand_frame_elim''.
-    + specialize (IHtg2 _ (Finite_Integer k, rroot) _ H). sep_apply IHtg2. clear.
-      rewrite distrib_orp_sepcon. apply orp_derives.
-      * Intros r. Exists r. cancel. rewrite <- wand_sepcon_adjoint.
-        cancel. apply wand_frame_elim''.
-      * Intros r x v0 ga gb i1 i2. Exists r x v0 ga gb i1 i2. cancel.
-        rewrite <- wand_sepcon_adjoint. cancel.
-        rewrite !sepcon_assoc. apply wand_frame_elim''.
-    + apply orp_right2. Exists (lroot, rroot) k v g g0. clear.
+  - rewrite -bi.or_intro_l. apply elem_of_singleton in H as ->. Exists r_root. cancel. apply wand_refl_cancel_right.
+  - destruct r_root as [lroot rroot]. rewrite !elem_of_union in H; destruct H as [[H | H] | H].
+    + apply elem_of_singleton in H as ->.
+      rewrite -bi.or_intro_r. Exists (lroot, rroot) k v g g0. clear.
       destruct tg1, tg2; simpl.
       * Exists (@None ghost_info) (@None ghost_info). cancel.
         apply wand_refl_cancel_right.
       * Exists (@None ghost_info) (Some (k0, v0, g1, g2)). cancel.
-        rewrite <- wand_sepcon_adjoint. cancel.
+        apply bi.wand_intro_r. cancel.
       * Exists (Some (k0, v0, g1, g2)) (@None ghost_info). cancel.
-        rewrite <- wand_sepcon_adjoint. cancel.
+        apply bi.wand_intro_r. cancel.
       * Exists (Some (k0, v0, g1, g2)) (Some (k1, v1, g3, g4)). cancel.
-        rewrite <- wand_sepcon_adjoint. cancel.
+        apply bi.wand_intro_r. cancel.
+    + specialize (IHtg1 _ (lroot, Finite_Integer k) _ H). sep_apply IHtg1. clear.
+      rewrite bi.sep_or_r; f_equiv.
+      * Intros r. Exists r. cancel. apply bi.wand_intro_r.
+        cancel. apply wand_frame_elim''.
+      * Intros r x v0 ga gb i1 i2. Exists r x v0 ga gb i1 i2. cancel.
+        apply bi.wand_intro_r. cancel.
+        rewrite -!sep_assoc. apply wand_frame_elim''.
+    + specialize (IHtg2 _ (Finite_Integer k, rroot) _ H). sep_apply IHtg2. clear.
+      rewrite bi.sep_or_r; f_equiv.
+      * Intros r. Exists r. cancel. apply bi.wand_intro_r.
+        cancel. apply wand_frame_elim''.
+      * Intros r x v0 ga gb i1 i2. Exists r x v0 ga gb i1 i2. cancel.
+        apply bi.wand_intro_r. cancel.
+        rewrite -!sep_assoc. apply wand_frame_elim''.
 Qed.
 
 Lemma range_info_in_tree_In: forall tg x v ga gb rn r_root,
-    range_info_in_tree (rn, Some (Some (x, v, ga, gb))) r_root tg ->
+    range_info_in_tree (rn, Excl' (Some (x, v, ga, gb))) r_root tg ->
     In_ghost x tg.
 Proof.
   induction tg; intros.
-  { inv H. inv H0. }
+  { inv H. }
   inv H.
-  - inv H1. now constructor 1.
+  - now constructor 1.
   - constructor 2. eapply IHtg1; eauto.
   - constructor 3. eapply IHtg2; eauto.
 Qed.
@@ -687,13 +628,13 @@ Qed.
 
 Lemma range_info_in_gmap: forall x v ga gb tg rn r_root,
     sorted_ghost_tree tg ->
-    range_info_in_tree (rn, Some (Some (x, v, ga, gb))) r_root tg ->
+    range_info_in_tree (rn, Excl' (Some (x, v, ga, gb))) r_root tg ->
     tree_to_gmap tg !! x = Some v.
 Proof.
   induction tg; intros; simpl.
-  { inv H0. inv H1. }
+  { inv H0. }
   inv H. inv H0.
-  - inv H1. apply lookup_insert.
+  - apply lookup_insert.
   - exploit Hgtl. { eapply range_info_in_tree_In; eauto. }
     intros; rewrite -> lookup_insert_ne by lia.
     eapply lookup_union_Some_l, IHtg1; eauto.
@@ -708,13 +649,12 @@ Qed.
 Lemma range_info_not_in_gmap: forall tg x rn r_root,
     sorted_ghost_tree tg -> key_in_range x rn = true ->
     keys_in_range_ghost tg r_root ->
-    range_info_in_tree (rn, Some None) r_root tg -> tree_to_gmap tg !! x = None.
+    range_info_in_tree (rn, Excl' None) r_root tg -> tree_to_gmap tg !! x = None.
 Proof.
   induction tg; intros; simpl.
   { apply lookup_empty. }
   apply keys_in_range_ghost_subtrees in H1 as (? & ? & ?); auto.
   inv H; inv H2.
-  - inv H5.
   - exploit range_info_incl; eauto; intros Hrange.
     pose proof (key_in_range_incl _ _ _ H0 Hrange) as Hx.
     apply andb_prop in Hx as []; simpl in *.
@@ -735,15 +675,14 @@ Qed.
 
 Lemma range_incl_tree_rep_R: forall tp r1 r2 g_info g,
     range_incl r1 r2 = true ->
-    tree_rep_R tp r1 g_info g |-- tree_rep_R tp r2 g_info g.
+    tree_rep_R tp r1 g_info g ⊢ tree_rep_R tp r2 g_info g.
 Proof.
-  intros. unfold tree_rep_R. if_tac. 1: cancel. Intros ga gb x v pa pb locka lockb.
-  Exists ga gb x v pa pb locka lockb. entailer!.
-  destruct (key_in_range x r1) eqn: ?. 2: easy.
+  intros. unfold tree_rep_R. if_tac. 1: cancel. do 16 f_equiv. entailer!.
+  destruct (key_in_range a1 r1) eqn: ?. 2: easy.
   eapply key_in_range_incl; eauto.
 Qed.
 
-Lemma node_info_incl: forall a b c,
+(*Lemma node_info_incl: forall a b c,
     @sepalg.join node_info (@Join_G node_ghost) a b c ->
     range_incl (fst a) (fst c) = true /\ match a.2 with Some x => c.2 = Some x | _ => True end.
 Proof.
@@ -765,7 +704,7 @@ Proof.
 Qed.
 
 Lemma public_sub : forall g sh a b,
-  my_half g sh a * public_half g b |-- 
+  my_half g sh a * public_half g b ⊢ 
     !! (range_incl (fst a) (fst b) = true /\ 
           match a.2 with 
           | Some x => b.2 = Some x 
@@ -788,9 +727,9 @@ Lemma in_tree_left_range:
     key_in_range x r.1 = true -> r.2 = Some (Some (x0, v, ga, gb)) -> Z.lt x x0 ->
     atomic_shift (λ M, tree_rep g g_root M) ⊤ ∅
                  b Q * my_half g_in gsh r * in_tree g g_in * my_half ga gsh1 a
-    |-- |={⊤}=> atomic_shift (λ M, tree_rep g g_root M) ⊤ ∅
+    ⊢ |={⊤}=> atomic_shift (λ M, tree_rep g g_root M) ⊤ ∅
     b Q * my_half g_in gsh r *
-    (EX ba, !! (less_than_equal ba r.1.1 = true /\
+    (∃ ba, !! (less_than_equal ba r.1.1 = true /\
                 range_incl a.1 (ba, Finite_Integer x0) = true) &&
             (in_tree g g_in * my_half ga gsh1 (ba, Finite_Integer x0, a.2))).
 
@@ -837,9 +776,9 @@ Lemma in_tree_right_range:
     key_in_range x r.1 = true -> r.2 = Some (Some (x0, v, ga, gb)) -> Z.lt x0 x ->
     atomic_shift (λ M, tree_rep g g_root M) ⊤ ∅
                  b Q * my_half g_in gsh r * in_tree g g_in * my_half gb gsh1 a
-    |-- |={⊤}=> atomic_shift (λ M, tree_rep g g_root M) ⊤ ∅
+    ⊢ |={⊤}=> atomic_shift (λ M, tree_rep g g_root M) ⊤ ∅
     b Q * my_half g_in gsh r *
-    (EX ta, !! (less_than_equal r.1.2 ta = true /\
+    (∃ ta, !! (less_than_equal r.1.2 ta = true /\
                 range_incl a.1 (Finite_Integer x0, ta) = true) &&
             (in_tree g g_in * my_half gb gsh1 (Finite_Integer x0, ta, a.2))).
 Proof.
@@ -884,33 +823,34 @@ Proof.
   - iIntros "[_ _]"; auto.
   - destruct r; iIntros "[[[_ _] HL] HR]".
     iPoseProof (IHtg1 with "HL") as "_"; iPoseProof (IHtg2 with "HR") as "_"; auto.
-Qed.
+Qed.*)
 
 Lemma ghost_tree_rep_public_half_ramif: forall tg g_root r_root g_in,
-    Ensembles.In (find_ghost_set tg g_root) g_in ->
-    ghost_tree_rep tg g_root r_root |--
-    EX r: node_info, !! (range_info_in_tree r r_root tg) &&
-      (public_half g_in r * (public_half g_in r -* ghost_tree_rep tg g_root r_root)).
+    g_in ∈ (find_ghost_set tg g_root) ->
+    ghost_tree_rep tg g_root r_root ⊢
+    ∃ r: node_info, ⌜range_info_in_tree r r_root tg⌝ ∧
+      (public_half g_in r ∗ (public_half g_in r -∗ ghost_tree_rep tg g_root r_root)).
 Proof.
   induction tg; intros; simpl in *.
-  - inv H. Exists (r_root, Some (@None ghost_info)). apply andp_right.
-    + apply prop_right. now constructor.
-    + cancel. apply wand_refl_cancel_right.
-  - destruct r_root as [l r]. inv H; inv H0.
+  - apply elem_of_singleton in H as ->. Exists (r_root, Excl' (@None ghost_info)). apply bi.and_intro.
+    + apply bi.pure_intro. now constructor.
+    + iIntros "$ $".
+  - destruct r_root as [l r]. rewrite !elem_of_union in H; destruct H as [[H | H] | H].
+    + apply elem_of_singleton in H as ->.
+      Exists (l, r, Excl' (Some (k, v, g, g0))). apply bi.and_intro.
+      * apply bi.pure_intro. now apply riit_root.
+      * cancel. iIntros "($ & $) $".
     + specialize (IHtg1 _ (l, Finite_Integer k) _ H). sep_apply IHtg1.
-      Intros r0. Exists r0. apply andp_right.
-      * apply prop_right. now apply riit_left.
-      * cancel. rewrite <- wand_sepcon_adjoint. cancel. apply wand_frame_elim''.
+      Intros r0. Exists r0. apply bi.and_intro.
+      * apply bi.pure_intro. now apply riit_left.
+      * cancel. apply bi.wand_intro_r. cancel. apply wand_frame_elim''.
     + specialize (IHtg2 _ (Finite_Integer k, r) _ H). sep_apply IHtg2.
-      Intros r0. Exists r0. apply andp_right.
-      * apply prop_right. now apply riit_right.
-      * cancel. rewrite <- wand_sepcon_adjoint. cancel. apply wand_frame_elim''.
-    + Exists (l, r, Some (Some (k, v, g, g0))). apply andp_right.
-      * apply prop_right. now apply riit_root.
-      * cancel. rewrite <- wand_sepcon_adjoint. cancel.
+      Intros r0. Exists r0. apply bi.and_intro.
+      * apply bi.pure_intro. now apply riit_right.
+      * cancel. apply bi.wand_intro_r. cancel. apply wand_frame_elim''.
 Qed.
 
-Lemma public_update : forall g (a b a' : G), my_half g gsh1 a * public_half g b |-- 
+(*Lemma public_update : forall g (a b a' : G), my_half g gsh1 a * public_half g b ⊢ 
   (|==> my_half g gsh1 a' * public_half g a')%I.
 Proof.
   intros; unfold public_half'.
@@ -930,3 +870,9 @@ Proof.
     * constructor.
   }
 Qed. *)
+
+End inv.
+
+Global Hint Resolve node_lock_inv_pred_exclusive : core.
+Global Hint Resolve empty_range_E : core.
+Global Hint Resolve keys_in_range_infinity : core.
